Veritas.Verifier.TSLog.fst
@@ -1746,6 +1746,9 @@ let lemma_init_state_empty (itsl: its_log {I.length itsl = 0}) (k: key)
     lemma_proj_length (partn eac_sm k empty) empty;
     assert (Seq.equal (partn eac_sm k empty) empty)
 
-let lemma_eac_value_init (itsl: eac_log) (k:key):
+let lemma_eac_value_init (itsl: eac_log) (k:key{k <> Root}):
   Lemma (requires (is_eac_state_init itsl k))
         (ensures (eac_value itsl k = init_value k)) = admit()
+
+let lemma_eac_value_root_init (itsl: eac_log {I.length itsl = 0}) (k:key{k = Root}):
+  Lemma (eac_value itsl k = init_value k)  = admit()
